compiler/backend/data_to_wordScript.sml
@@ -1,7 +1,7 @@
-open preamble wordLangTheory bvpTheory word_to_wordTheory;
+open preamble wordLangTheory dataLangTheory word_to_wordTheory;
 local open bvl_to_bviTheory in end
 
-val _ = new_theory "bvp_to_word";
+val _ = new_theory "data_to_word";
 
 val _ = Datatype `
   config = <| tag_bits : num (* in each pointer *)
@@ -33,7 +33,7 @@ val tag_mask_def = Define `
       (l-1 '' 2) (~0w:'a word)`
 
 val encode_header_def = Define `
-  encode_header (conf:bvp_to_word$config) tag len =
+  encode_header (conf:data_to_word$config) tag len =
     if tag < 2 ** (dimindex (:'a) - conf.len_size - 2) /\
        tag < dimword (:'a) DIV 16 /\
        len < 2 ** (dimindex (:'a) - 4) /\
@@ -76,7 +76,7 @@ val ptr_bits_def = Define `
      maxout_bits len conf.len_bits 1)`
 
 val real_addr_def = Define `
-  (real_addr (conf:bvp_to_word$config) r): 'a wordLang$exp =
+  (real_addr (conf:data_to_word$config) r): 'a wordLang$exp =
     let k = shift (:'a) in
    (* if k <= conf.pad_bits + 1 then
         Op Add [Lookup CurrHeap;
@@ -87,7 +87,7 @@ val real_addr_def = Define `
                   (Nat (shift_length conf))) (Nat k)]`
 
 val real_offset_def = Define `
-  (real_offset (conf:bvp_to_word$config) r): 'a wordLang$exp =
+  (real_offset (conf:data_to_word$config) r): 'a wordLang$exp =
      Op Add [Const bytes_in_word;
              if dimindex (:'a) = 32 then Var r else Shift Lsl (Var r) (Nat 1)]`
 
@@ -138,7 +138,7 @@ val RefByte_code_def = Define`
     Call NONE (SOME RefByte_location) [2;4;6] NONE])`;
 
 val assign_def = Define `
-  assign (c:bvp_to_word$config) (secn:num) (l:num) (dest:num) (op:closLang$op)
+  assign (c:data_to_word$config) (secn:num) (l:num) (dest:num) (op:closLang$op)
     (args:num list) (names:num_set option) =
     case op of
     | Const i =>
@@ -502,7 +502,7 @@ val assign_def = Define `
     | _ => (GiveUp:'a wordLang$prog,l)`;
 
 val comp_def = Define `
-  comp c (secn:num) (l:num) (p:bvp$prog) =
+  comp c (secn:num) (l:num) (p:dataLang$prog) =
     case p of
     | Skip => (Skip:'a wordLang$prog,l)
     | Tick => (Tick,l)
@@ -549,12 +549,12 @@ val stubs_def = Define`
   ]`;
 
 val check_stubs_length = Q.store_thm("check_stubs_length",
-  `wordLang$num_stubs + LENGTH (stubs (:α)) = bvp$num_stubs`,
+  `wordLang$num_stubs + LENGTH (stubs (:α)) = dataLang$num_stubs`,
   EVAL_TAC);
 
 val compile_def = Define `
-  compile bvp_conf word_conf asm_conf prog =
-    let p = stubs (:α) ++ MAP (compile_part bvp_conf) prog in
+  compile data_conf word_conf asm_conf prog =
+    let p = stubs (:α) ++ MAP (compile_part data_conf) prog in
       word_to_word$compile word_conf (asm_conf:'a asm_config) p`;
 
 val _ = export_theory();
