compiler/backend/dataLangScript.sml
@@ -1,11 +1,11 @@
 open preamble;
 local open bvlTheory wordLangTheory in end;
 
-val _ = new_theory "bvp";
+val _ = new_theory "dataLang";
 
-(* BVP = bytecode-value program *)
+(* dataLang = last language with a data abstraction *)
 
-(* BVP is the next step from BVL: (1) BVP is an imperative version of
+(* dataLang is the next step from BVL: (1) dataLang is an imperative version of
    BVL, i.e. operations update state; (2) there is a new state
    component (called space) and an explicit MakeSpace operation that
    increases space. Space is consumed by Ref and Cons. *)
@@ -19,14 +19,14 @@ val _ = new_theory "bvp";
 (* The MakeSpace command has an optional variable name list. If this
    list is provided, i.e. SOME var_names, then only these variables
    can survive the execution of the MakeSpace command. The idea is
-   that one generates MakeSpace X NONE when compiling into BVP. Then
+   that one generates MakeSpace X NONE when compiling into dataLang. Then
    optimisations move around and combine MakeSpace commands. Then
    liveness analysis annotates each MakeSpace command with a SOME. The
-   translation from BVP into more concete forms must implement a GC
+   translation from dataLang into more concete forms must implement a GC
    that only looks at the variables in the SOME annotations. *)
 
 
-(* --- Syntax of BVP --- *)
+(* --- Syntax of dataLang --- *)
 
 val _ = Datatype `
   prog = Skip
@@ -34,10 +34,10 @@ val _ = Datatype `
        | Call ((num # num_set) option) (* return var, cut-set *)
                           (num option) (* target of call *)
                             (num list) (* arguments *)
-             ((num # bvp$prog) option) (* handler: varname, handler code *)
+             ((num # dataLang$prog) option) (* handler: varname, handler code *)
        | Assign num op (num list) (num_set option)
-       | Seq bvp$prog bvp$prog
-       | If num bvp$prog bvp$prog
+       | Seq dataLang$prog dataLang$prog
+       | If num dataLang$prog dataLang$prog
        | MakeSpace num num_set
        | Raise num
        | Return num
