compiler/eval/x64/x64_configScript.sml
@@ -10,7 +10,7 @@ val source_conf = rconc(EVAL``prim_config.source_conf``)
 val mod_conf = rconc(EVAL``prim_config.mod_conf``)
 (* Note: prim_config condition in backend needs to be relaxed *)
 val clos_conf = rconc (EVAL ``prim_config.clos_conf with <|do_mti:=T;do_known:=T;do_call:=T;do_remove:=T|>``)
-val bvp_conf = ``<| tag_bits:=4; len_bits:=4; pad_bits:=0; len_size:=16|>``
+val data_conf = ``<| tag_bits:=4; len_bits:=4; pad_bits:=0; len_size:=16|>``
 val word_to_word_conf = ``<| reg_alg:=1; col_oracle := λn. NONE |>``
 (*val word_conf = ``<| bitmaps := [] |>``*)
 val stack_conf = ``<|reg_names:=x64_names;max_heap:=1000000|>``
@@ -21,7 +21,7 @@ val x64_compiler_config_def = Define`
              <|source_conf:=^(source_conf);
                mod_conf:=^(mod_conf);
                clos_conf:=^(clos_conf);
-               bvp_conf:=^(bvp_conf);
+               data_conf:=^(data_conf);
                word_to_word_conf:=^(word_to_word_conf);
                (*word_conf:=^(word_conf);*)
                stack_conf:=^(stack_conf);
