compiler/proofs/compilerProofScript.sml
@@ -126,7 +126,7 @@ val compile_correct_gen = Q.store_thm("compile_correct_gen",
           installed (bytes,cc.backend_config,st.sem_st.ffi,ffi_limit,mc,ms) ⇒
             machine_sem mc st.sem_st.ffi ms ⊆
               extend_with_resource_limit behaviours
-              (* see theorem about to_bvp to avoid extend_with_resource_limit *)`,
+              (* see theorem about to_data to avoid extend_with_resource_limit *)`,
   rpt strip_tac
   \\ simp[compilerTheory.compile_def]
   \\ simp[parse_prog_correct]
@@ -198,7 +198,7 @@ val compile_correct = Q.store_thm("compile_correct",
           code_installed (bytes,cc,ffi,ffi_limit,mc,ms) ⇒
             machine_sem mc ffi ms ⊆
               extend_with_resource_limit behaviours
-              (* see theorem about to_bvp to avoid extend_with_resource_limit *)`,
+              (* see theorem about to_data to avoid extend_with_resource_limit *)`,
   rw[initSemEnvTheory.semantics_init_def,code_installed_def]
   \\ qmatch_goalsub_abbrev_tac`semantics$semantics st`
   \\ `(FST(THE(prim_sem_env ffi))).ffi = ffi` by simp[initSemEnvTheory.prim_sem_env_eq]
